src/Denotational.thy
@@ -28,10 +28,12 @@ fun TESL_interpretation_atomic
                           \<and> time ((Rep_run \<rho>) m measuring) = measured_time + \<delta>\<tau>
                  )
         }"
-  | "\<lbrakk> K\<^sub>1 precedes K\<^sub>2 \<rbrakk>\<^sub>T\<^sub>E\<^sub>S\<^sub>L =
+  | "\<lbrakk> K\<^sub>1 weakly precedes K\<^sub>2 \<rbrakk>\<^sub>T\<^sub>E\<^sub>S\<^sub>L =
         { \<rho>. \<forall>n::nat. (run_tick_count \<rho> K\<^sub>2 n) \<le> (run_tick_count_strictly \<rho> K\<^sub>1 n) }"
   | "\<lbrakk> K\<^sub>1 strictly precedes K\<^sub>2 \<rbrakk>\<^sub>T\<^sub>E\<^sub>S\<^sub>L =
         { \<rho>. \<forall>n::nat. (run_tick_count \<rho> K\<^sub>2 n) < (run_tick_count_strictly \<rho> K\<^sub>1 n) }"
+  | "\<lbrakk> K\<^sub>1 kills K\<^sub>2 \<rbrakk>\<^sub>T\<^sub>E\<^sub>S\<^sub>L =
+        { \<rho>. \<forall>n::nat. hamlet ((Rep_run \<rho>) n K\<^sub>1) \<longrightarrow> (\<forall>m\<ge>n. \<not> hamlet ((Rep_run \<rho>) m K\<^sub>2)) }"
 
 section \<open>Denotational interpretation for TESL formulae\<close>
 
