src/TESL.thy
@@ -49,8 +49,9 @@ datatype '\<tau> TESL_atomic =
   | Implies        "clock" "clock"                         (infixr "implies" 55)
   | ImpliesNot     "clock" "clock"                         (infixr "implies not" 55)
   | TimeDelayedBy  "clock" "'\<tau> tag_const" "clock" "clock"     ("_ time-delayed by _ on _ implies _" 55)
-  | Precedes       "clock" "clock"                         (infixr "precedes" 55)
+  | WeaklyPrecedes "clock" "clock"                         (infixr "weakly precedes" 55)
   | StrictlyPrecedes "clock" "clock"                       (infixr "strictly precedes" 55)
+  | Kills          "clock" "clock"                         (infixr "kills" 55)
 
 type_synonym '\<tau> TESL_formula = "'\<tau> TESL_atomic list"
 
